FloatModel/Float.lean
@@ -11,5 +11,4 @@ public import FloatModel.Float.Round
 public import FloatModel.Float.Pack
 public import FloatModel.Float.Operations
 public import FloatModel.Float.Model
-public import FloatModel.Float.Valid
 public import FloatModel.Float.Lemmas
