FloatModel/Float/Lemmas.lean
@@ -5,31 +5,49 @@ Authors: Julia M. Himmel
 -/
 module
 
-public import FloatModel.Float.Valid
-public import FloatModel.Float.Round
+public import FloatModel.Float.Model
 
 namespace FloatModel
 
 @[simp]
-theorem snd_shiftToTargetExponent {spec : FloatSpec} {mantissa : Nat} {exponent : Int}
-    {accuracy : Accuracy} :
-    (shiftToTargetExponent spec mantissa exponent accuracy).2 = max exponent (spec.targetExponent (totalExponent mantissa exponent)) := by
-  grind [shiftToTargetExponent]
+theorem unpackMantissa_packComponents {spec : FloatSpec} {sign exponent mantissa} :
+    unpackMantissa (packComponents spec sign exponent mantissa) = mantissa := by
+  ext i hi
+  simp [unpackMantissa, packComponents, BitVec.getLsbD_eq_getElem, BitVec.getLsbD_append, hi]
 
-theorem totalExponent_shiftToTargetExponent {spec : FloatSpec} {mantissa : Nat} {exponent : Int}
-    {accuracy : Accuracy} :
-    totalExponent (shiftToTargetExponent spec mantissa exponent accuracy).1.mantissa (shiftToTargetExponent spec mantissa exponent accuracy).2 =
-    totalExponent mantissa exponent := by
-  sorry
+@[simp]
+theorem unpackExponent_packComponents {spec : FloatSpec} {sign exponent mantissa} :
+    unpackExponent (packComponents spec sign exponent mantissa) = exponent := by
+  ext i hi
+  simp [unpackExponent, packComponents, BitVec.getLsbD_eq_getElem, BitVec.getLsbD_append, hi]
 
-theorem valid_roundWithAccuracy {spec : FloatSpec} {sign : Sign} {mantissa : Nat} {exponent : Int}
-    {accuracy : Accuracy} (h : exponent ≤ spec.targetExponent (totalExponent mantissa exponent)) :
-    spec.Valid (roundWithAccuracy spec sign mantissa exponent accuracy) := by
-  fun_cases roundWithAccuracy with
+@[simp]
+theorem BitVec.zero_eq_neg_one_iff {w : Nat} : 0#w = (-1#w) ↔ w = 0 := by
+  simp [← BitVec.toNat_inj]
+  match w with
+  | 0 => simp
+  | w + 1 =>
+    suffices 0 ≠ 2 ^ (w + 1) - 1 by simpa
+    have : 2 ≤ 2 ^ (w + 1) := Nat.le_pow (by simp)
+    omega
+
+theorem valid_pack {spec : FloatSpec} {f : UnpackedFloat} : spec.Valid (pack spec f) := by
+  refine ⟨?_⟩
+  fun_cases pack with
   | case1 => simp
-  | case2 em₁ e₁ hshift roundedEm₁ finalExtendedMantissa finalExponent hshift' finalMantissa hne =>
-    refine .finite _ _ _ _ ⟨?_, ?_⟩
-    · sorry
-    · sorry
+  | case2 s => simp [packedInfinity]
+  | case3 s => simp [packedZero]
+  | case4 s m e hm biasedExponent h => simp [packedInfinity]
+  | case5 s m e hm actualMantissaBits biasedExponent h₁ h₂ =>
+    suffices biasedExponent % 2 ^ spec.exponentBits ≠ 2 ^ spec.exponentBits - 1 by
+      simp [BitVec.neg_one_eq_allOnes, ← BitVec.toNat_inj, this]
+    clear h₂ actualMantissaBits hm m s
+    suffices biasedExponent < 2 ^ spec.exponentBits - 1 by
+      intro h
+      rw [Nat.mod_eq_of_lt (by omega)] at h
+      omega
+    omega
+  | case6 s m e hm actualMantissaBits biasedExponent h₁ h₂ =>
+    simp [Nat.pos_iff_ne_zero.1 spec.he]
 
 end FloatModel
